feat: rename `List.enum(From)` to `List.zipIdx`, and `Array/Vector.zipWithIndex` to `zipIdx` (#6800)
This PR uniformizes the naming of `enum`/`enumFrom` (on `List`) and
`zipWithIndex` (on `Array` on `Vector`), replacing all with `zipIdx`. At
the same time, we generalize to add an optional `Nat` parameter for the
initial value of the index (which previously existed, only for `List`,
as the separate function `enumFrom`).

src/Init/Data/Array/Basic.lean
@@ -605,8 +605,10 @@ def mapIdx {α : Type u} {β : Type v} (f : Nat → α → β) (as : Array α) :
   Id.run <| as.mapIdxM f
 
 /-- Turns `#[a, b]` into `#[(a, 0), (b, 1)]`. -/
-def zipWithIndex (arr : Array α) : Array (α × Nat) :=
-  arr.mapIdx fun i a => (a, i)
+def zipIdx (arr : Array α) (start := 0) : Array (α × Nat) :=
+  arr.mapIdx fun i a => (a, i + start)
+
+@[deprecated zipIdx (since := "2025-01-21")] abbrev zipWithIndex := @zipIdx
 
 @[inline]
 def find? {α : Type u} (p : α → Bool) (as : Array α) : Option α :=
