src/Init/Data/List/Nat/Range.lean
@@ -339,25 +339,166 @@ theorem find?_iota_eq_some {n : Nat} {i : Nat} {p : Nat → Bool} :
 
 end
 
-/-! ### enumFrom -/
+/-! ### zipIdx -/
 
 @[simp]
+theorem zipIdx_singleton (x : α) (k : Nat) : zipIdx [x] k = [(x, k)] :=
+  rfl
+
+@[simp] theorem head?_zipIdx (l : List α) (k : Nat) :
+    (zipIdx l k).head? = l.head?.map fun a => (a, k) := by
+  simp [head?_eq_getElem?]
+
+@[simp] theorem getLast?_zipIdx (l : List α) (k : Nat) :
+    (zipIdx l k).getLast? = l.getLast?.map fun a => (a, k + l.length - 1) := by
+  simp [getLast?_eq_getElem?]
+  cases l <;> simp; omega
+
+theorem mk_add_mem_zipIdx_iff_getElem? {k i : Nat} {x : α} {l : List α} :
+    (x, k + i) ∈ zipIdx l k ↔ l[i]? = some x := by
+  simp [mem_iff_getElem?, and_left_comm]
+
+theorem mk_mem_zipIdx_iff_le_and_getElem?_sub {k i : Nat} {x : α} {l : List α} :
+    (x, i) ∈ zipIdx l k ↔ k ≤ i ∧ l[i - k]? = some x := by
+  if h : k ≤ i then
+    rcases Nat.exists_eq_add_of_le h with ⟨i, rfl⟩
+    simp [mk_add_mem_zipIdx_iff_getElem?, Nat.add_sub_cancel_left]
+  else
+    have : ∀ m, k + m ≠ i := by rintro _ rfl; simp at h
+    simp [h, mem_iff_get?, this]
+
+/-- Variant of `mk_mem_zipIdx_iff_le_and_getElem?_sub` specialized at `k = 0`,
+to avoid the inequality and the subtraction. -/
+theorem mk_mem_zipIdx_iff_getElem? {i : Nat} {x : α} {l : List α} : (x, i) ∈ zipIdx l ↔ l[i]? = x := by
+  simp [mk_mem_zipIdx_iff_le_and_getElem?_sub]
+
+theorem mem_zipIdx_iff_le_and_getElem?_sub {x : α × Nat} {l : List α} {k : Nat} :
+    x ∈ zipIdx l k ↔ k ≤ x.2 ∧ l[x.2 - k]? = some x.1 := by
+  cases x
+  simp [mk_mem_zipIdx_iff_le_and_getElem?_sub]
+
+/-- Variant of `mem_zipIdx_iff_le_and_getElem?_sub` specialized at `k = 0`,
+to avoid the inequality and the subtraction. -/
+theorem mem_zipIdx_iff_getElem? {x : α × Nat} {l : List α} : x ∈ zipIdx l ↔ l[x.2]? = some x.1 := by
+  cases x
+  simp [mk_mem_zipIdx_iff_le_and_getElem?_sub]
+
+theorem le_snd_of_mem_zipIdx {x : α × Nat} {k : Nat} {l : List α} (h : x ∈ zipIdx l k) :
+    k ≤ x.2 :=
+  (mk_mem_zipIdx_iff_le_and_getElem?_sub.1 h).1
+
+theorem snd_lt_add_of_mem_zipIdx {x : α × Nat} {l : List α} {k : Nat} (h : x ∈ zipIdx l k) :
+    x.2 < k + length l := by
+  rcases mem_iff_get.1 h with ⟨i, rfl⟩
+  simpa using i.isLt
+
+theorem snd_lt_of_mem_zipIdx {x : α × Nat} {l : List α} {k : Nat} (h : x ∈ l.zipIdx k) : x.2 < l.length + k := by
+  simpa [Nat.add_comm] using snd_lt_add_of_mem_zipIdx h
+
+theorem map_zipIdx (f : α → β) (l : List α) (k : Nat) :
+    map (Prod.map f id) (zipIdx l k) = zipIdx (l.map f) k := by
+  induction l generalizing k <;> simp_all
+
+theorem fst_mem_of_mem_zipIdx {x : α × Nat} {l : List α} {k : Nat} (h : x ∈ zipIdx l k) : x.1 ∈ l :=
+  zipIdx_map_fst k l ▸ mem_map_of_mem _ h
+
+theorem fst_eq_of_mem_zipIdx {x : α × Nat} {l : List α} {k : Nat} (h : x ∈ zipIdx l k) :
+    x.1 = l[x.2 - k]'(by have := le_snd_of_mem_zipIdx h; have := snd_lt_add_of_mem_zipIdx h; omega) := by
+  induction l generalizing k with
+  | nil => cases h
+  | cons hd tl ih =>
+    cases h with
+    | head h => simp
+    | tail h m =>
+      specialize ih m
+      have : x.2 - k = x.2 - (k + 1) + 1 := by
+        have := le_snd_of_mem_zipIdx m
+        omega
+      simp [this, ih]
+
+theorem mem_zipIdx {x : α} {i : Nat} {xs : List α} {k : Nat} (h : (x, i) ∈ xs.zipIdx k) :
+    k ≤ i ∧ i < k + xs.length ∧
+      x = xs[i - k]'(by have := le_snd_of_mem_zipIdx h; have := snd_lt_add_of_mem_zipIdx h; omega) :=
+  ⟨le_snd_of_mem_zipIdx h, snd_lt_add_of_mem_zipIdx h, fst_eq_of_mem_zipIdx h⟩
+
+/-- Variant of `mem_zipIdx` specialized at `k = 0`. -/
+theorem mem_zipIdx' {x : α} {i : Nat} {xs : List α} (h : (x, i) ∈ xs.zipIdx) :
+    i < xs.length ∧ x = xs[i]'(by have := le_snd_of_mem_zipIdx h; have := snd_lt_add_of_mem_zipIdx h; omega) :=
+  ⟨by simpa using snd_lt_add_of_mem_zipIdx h, fst_eq_of_mem_zipIdx h⟩
+
+theorem zipIdx_map (l : List α) (k : Nat) (f : α → β) :
+    zipIdx (l.map f) k = (zipIdx l k).map (Prod.map f id) := by
+  induction l with
+  | nil => rfl
+  | cons hd tl IH =>
+    rw [map_cons, zipIdx_cons', zipIdx_cons', map_cons, map_map, IH, map_map]
+    rfl
+
+theorem zipIdx_append (xs ys : List α) (k : Nat) :
+    zipIdx (xs ++ ys) k = zipIdx xs k ++ zipIdx ys (k + xs.length) := by
+  induction xs generalizing ys k with
+  | nil => simp
+  | cons x xs IH =>
+    rw [cons_append, zipIdx_cons, IH, ← cons_append, ← zipIdx_cons, length, Nat.add_right_comm,
+      Nat.add_assoc]
+
+theorem zipIdx_eq_cons_iff {l : List α} {k : Nat} :
+    zipIdx l k = x :: l' ↔ ∃ a as, l = a :: as ∧ x = (a, k) ∧ l' = zipIdx as (k + 1) := by
+  rw [zipIdx_eq_zip_range', zip_eq_cons_iff]
+  constructor
+  · rintro ⟨l₁, l₂, rfl, h, rfl⟩
+    rw [range'_eq_cons_iff] at h
+    obtain ⟨rfl, -, rfl⟩ := h
+    exact ⟨x.1, l₁, by simp [zipIdx_eq_zip_range']⟩
+  · rintro ⟨a, as, rfl, rfl, rfl⟩
+    refine ⟨as, range' (k+1) as.length, ?_⟩
+    simp [zipIdx_eq_zip_range', range'_succ]
+
+theorem zipIdx_eq_append_iff {l : List α} {k : Nat} :
+    zipIdx l k = l₁ ++ l₂ ↔
+      ∃ l₁' l₂', l = l₁' ++ l₂' ∧ l₁ = zipIdx l₁' k ∧ l₂ = zipIdx l₂' (k + l₁'.length) := by
+  rw [zipIdx_eq_zip_range', zip_eq_append_iff]
+  constructor
+  · rintro ⟨w, x, y, z, h, rfl, h', rfl, rfl⟩
+    rw [range'_eq_append_iff] at h'
+    obtain ⟨k, -, rfl, rfl⟩ := h'
+    simp only [length_range'] at h
+    obtain rfl := h
+    refine ⟨w, x, rfl, ?_⟩
+    simp only [zipIdx_eq_zip_range', length_append, true_and]
+    congr
+    omega
+  · rintro ⟨l₁', l₂', rfl, rfl, rfl⟩
+    simp only [zipIdx_eq_zip_range']
+    refine ⟨l₁', l₂', range' k l₁'.length, range' (k + l₁'.length) l₂'.length, ?_⟩
+    simp [Nat.add_comm]
+
+/-! ### enumFrom -/
+
+section
+set_option linter.deprecated false
+
+@[deprecated zipIdx_singleton (since := "2025-01-21"), simp]
 theorem enumFrom_singleton (x : α) (n : Nat) : enumFrom n [x] = [(n, x)] :=
   rfl
 
-@[simp] theorem head?_enumFrom (n : Nat) (l : List α) :
+@[deprecated head?_zipIdx (since := "2025-01-21"), simp]
+theorem head?_enumFrom (n : Nat) (l : List α) :
     (enumFrom n l).head? = l.head?.map fun a => (n, a) := by
   simp [head?_eq_getElem?]
 
-@[simp] theorem getLast?_enumFrom (n : Nat) (l : List α) :
+@[deprecated getLast?_zipIdx (since := "2025-01-21"), simp]
+theorem getLast?_enumFrom (n : Nat) (l : List α) :
     (enumFrom n l).getLast? = l.getLast?.map fun a => (n + l.length - 1, a) := by
   simp [getLast?_eq_getElem?]
   cases l <;> simp; omega
 
+@[deprecated mk_add_mem_zipIdx_iff_getElem? (since := "2025-01-21")]
 theorem mk_add_mem_enumFrom_iff_getElem? {n i : Nat} {x : α} {l : List α} :
     (n + i, x) ∈ enumFrom n l ↔ l[i]? = some x := by
   simp [mem_iff_get?]
 
+@[deprecated mk_mem_zipIdx_iff_le_and_getElem?_sub (since := "2025-01-21")]
 theorem mk_mem_enumFrom_iff_le_and_getElem?_sub {n i : Nat} {x : α} {l : List α} :
     (i, x) ∈ enumFrom n l ↔ n ≤ i ∧ l[i - n]? = x := by
   if h : n ≤ i then
@@ -367,22 +508,27 @@ theorem mk_mem_enumFrom_iff_le_and_getElem?_sub {n i : Nat} {x : α} {l : List �
     have : ∀ k, n + k ≠ i := by rintro k rfl; simp at h
     simp [h, mem_iff_get?, this]
 
+@[deprecated le_snd_of_mem_zipIdx (since := "2025-01-21")]
 theorem le_fst_of_mem_enumFrom {x : Nat × α} {n : Nat} {l : List α} (h : x ∈ enumFrom n l) :
     n ≤ x.1 :=
   (mk_mem_enumFrom_iff_le_and_getElem?_sub.1 h).1
 
+@[deprecated snd_lt_add_of_mem_zipIdx (since := "2025-01-21")]
 theorem fst_lt_add_of_mem_enumFrom {x : Nat × α} {n : Nat} {l : List α} (h : x ∈ enumFrom n l) :
     x.1 < n + length l := by
   rcases mem_iff_get.1 h with ⟨i, rfl⟩
   simpa using i.isLt
 
+@[deprecated map_zipIdx (since := "2025-01-21")]
 theorem map_enumFrom (f : α → β) (n : Nat) (l : List α) :
     map (Prod.map id f) (enumFrom n l) = enumFrom n (map f l) := by
   induction l generalizing n <;> simp_all
 
+@[deprecated fst_mem_of_mem_zipIdx (since := "2025-01-21")]
 theorem snd_mem_of_mem_enumFrom {x : Nat × α} {n : Nat} {l : List α} (h : x ∈ enumFrom n l) : x.2 ∈ l :=
   enumFrom_map_snd n l ▸ mem_map_of_mem _ h
 
+@[deprecated fst_eq_of_mem_zipIdx (since := "2025-01-21")]
 theorem snd_eq_of_mem_enumFrom {x : Nat × α} {n : Nat} {l : List α} (h : x ∈ enumFrom n l) :
     x.2 = l[x.1 - n]'(by have := le_fst_of_mem_enumFrom h; have := fst_lt_add_of_mem_enumFrom h; omega) := by
   induction l generalizing n with
@@ -397,11 +543,13 @@ theorem snd_eq_of_mem_enumFrom {x : Nat × α} {n : Nat} {l : List α} (h : x �
         omega
       simp [this, ih]
 
+@[deprecated mem_zipIdx (since := "2025-01-21")]
 theorem mem_enumFrom {x : α} {i j : Nat} {xs : List α} (h : (i, x) ∈ xs.enumFrom j) :
     j ≤ i ∧ i < j + xs.length ∧
       x = xs[i - j]'(by have := le_fst_of_mem_enumFrom h; have := fst_lt_add_of_mem_enumFrom h; omega) :=
   ⟨le_fst_of_mem_enumFrom h, fst_lt_add_of_mem_enumFrom h, snd_eq_of_mem_enumFrom h⟩
 
+@[deprecated zipIdx_map (since := "2025-01-21")]
 theorem enumFrom_map (n : Nat) (l : List α) (f : α → β) :
     enumFrom n (l.map f) = (enumFrom n l).map (Prod.map id f) := by
   induction l with
@@ -410,6 +558,7 @@ theorem enumFrom_map (n : Nat) (l : List α) (f : α → β) :
     rw [map_cons, enumFrom_cons', enumFrom_cons', map_cons, map_map, IH, map_map]
     rfl
 
+@[deprecated zipIdx_append (since := "2025-01-21")]
 theorem enumFrom_append (xs ys : List α) (n : Nat) :
     enumFrom n (xs ++ ys) = enumFrom n xs ++ enumFrom (n + xs.length) ys := by
   induction xs generalizing ys n with
@@ -418,6 +567,7 @@ theorem enumFrom_append (xs ys : List α) (n : Nat) :
     rw [cons_append, enumFrom_cons, IH, ← cons_append, ← enumFrom_cons, length, Nat.add_right_comm,
       Nat.add_assoc]
 
+@[deprecated zipIdx_eq_cons_iff (since := "2025-01-21")]
 theorem enumFrom_eq_cons_iff {l : List α} {n : Nat} :
     l.enumFrom n = x :: l' ↔ ∃ a as, l = a :: as ∧ x = (n, a) ∧ l' = enumFrom (n + 1) as := by
   rw [enumFrom_eq_zip_range', zip_eq_cons_iff]
@@ -430,6 +580,7 @@ theorem enumFrom_eq_cons_iff {l : List α} {n : Nat} :
     refine ⟨range' (n+1) as.length, as, ?_⟩
     simp [enumFrom_eq_zip_range', range'_succ]
 
+@[deprecated zipIdx_eq_append_iff (since := "2025-01-21")]
 theorem enumFrom_eq_append_iff {l : List α} {n : Nat} :
     l.enumFrom n = l₁ ++ l₂ ↔
       ∃ l₁' l₂', l = l₁' ++ l₂' ∧ l₁ = l₁'.enumFrom n ∧ l₂ = l₂'.enumFrom (n + l₁'.length) := by
@@ -449,89 +600,113 @@ theorem enumFrom_eq_append_iff {l : List α} {n : Nat} :
     refine ⟨range' n l₁'.length, range' (n + l₁'.length) l₂'.length, l₁', l₂', ?_⟩
     simp [Nat.add_comm]
 
+end
+
 /-! ### enum -/
 
-@[simp]
+section
+set_option linter.deprecated false
+
+@[deprecated zipIdx_eq_nil_iff (since := "2025-01-21"), simp]
 theorem enum_eq_nil_iff {l : List α} : List.enum l = [] ↔ l = [] := enumFrom_eq_nil
 
-@[deprecated enum_eq_nil_iff (since := "2024-11-04")]
+@[deprecated zipIdx_eq_nil_iff (since := "2024-11-04")]
 theorem enum_eq_nil {l : List α} : List.enum l = [] ↔ l = [] := enum_eq_nil_iff
 
-@[simp] theorem enum_singleton (x : α) : enum [x] = [(0, x)] := rfl
+@[deprecated zipIdx_singleton (since := "2025-01-21"), simp]
+theorem enum_singleton (x : α) : enum [x] = [(0, x)] := rfl
 
-@[simp] theorem enum_length : (enum l).length = l.length :=
+@[deprecated length_zipIdx (since := "2025-01-21"), simp]
+theorem enum_length : (enum l).length = l.length :=
   enumFrom_length
 
-@[simp]
+@[deprecated getElem?_zipIdx (since := "2025-01-21"), simp]
 theorem getElem?_enum (l : List α) (n : Nat) : (enum l)[n]? = l[n]?.map fun a => (n, a) := by
   rw [enum, getElem?_enumFrom, Nat.zero_add]
 
-@[simp]
+@[deprecated getElem_zipIdx (since := "2025-01-21"), simp]
 theorem getElem_enum (l : List α) (i : Nat) (h : i < l.enum.length) :
     l.enum[i] = (i, l[i]'(by simpa [enum_length] using h)) := by
   simp [enum]
 
-@[simp] theorem head?_enum (l : List α) :
+@[deprecated head?_zipIdx (since := "2025-01-21"), simp] theorem head?_enum (l : List α) :
     l.enum.head? = l.head?.map fun a => (0, a) := by
   simp [head?_eq_getElem?]
 
-@[simp] theorem getLast?_enum (l : List α) :
+@[deprecated getLast?_zipIdx (since := "2025-01-21"), simp]
+theorem getLast?_enum (l : List α) :
     l.enum.getLast? = l.getLast?.map fun a => (l.length - 1, a) := by
   simp [getLast?_eq_getElem?]
 
-@[simp] theorem tail_enum (l : List α) : (enum l).tail = enumFrom 1 l.tail := by
+@[deprecated tail_zipIdx (since := "2025-01-21"), simp]
+theorem tail_enum (l : List α) : (enum l).tail = enumFrom 1 l.tail := by
   simp [enum]
 
+@[deprecated mk_mem_zipIdx_iff_getElem? (since := "2025-01-21")]
 theorem mk_mem_enum_iff_getElem? {i : Nat} {x : α} {l : List α} : (i, x) ∈ enum l ↔ l[i]? = x := by
   simp [enum, mk_mem_enumFrom_iff_le_and_getElem?_sub]
 
+@[deprecated mem_zipIdx_iff_getElem? (since := "2025-01-21")]
 theorem mem_enum_iff_getElem? {x : Nat × α} {l : List α} : x ∈ enum l ↔ l[x.1]? = some x.2 :=
   mk_mem_enum_iff_getElem?
 
+@[deprecated snd_lt_of_mem_zipIdx (since := "2025-01-21")]
 theorem fst_lt_of_mem_enum {x : Nat × α} {l : List α} (h : x ∈ enum l) : x.1 < length l := by
   simpa using fst_lt_add_of_mem_enumFrom h
 
+@[deprecated fst_mem_of_mem_zipIdx (since := "2025-01-21")]
 theorem snd_mem_of_mem_enum {x : Nat × α} {l : List α} (h : x ∈ enum l) : x.2 ∈ l :=
   snd_mem_of_mem_enumFrom h
 
+@[deprecated fst_eq_of_mem_zipIdx (since := "2025-01-21")]
 theorem snd_eq_of_mem_enum {x : Nat × α} {l : List α} (h : x ∈ enum l) :
     x.2 = l[x.1]'(fst_lt_of_mem_enum h) :=
   snd_eq_of_mem_enumFrom h
 
+@[deprecated mem_zipIdx (since := "2025-01-21")]
 theorem mem_enum {x : α} {i : Nat} {xs : List α} (h : (i, x) ∈ xs.enum) :
     i < xs.length ∧ x = xs[i]'(fst_lt_of_mem_enum h) :=
   by simpa using mem_enumFrom h
 
+@[deprecated map_zipIdx (since := "2025-01-21")]
 theorem map_enum (f : α → β) (l : List α) : map (Prod.map id f) (enum l) = enum (map f l) :=
   map_enumFrom f 0 l
 
-@[simp] theorem enum_map_fst (l : List α) : map Prod.fst (enum l) = range l.length := by
+@[deprecated zipIdx_map_snd (since := "2025-01-21"), simp]
+theorem enum_map_fst (l : List α) : map Prod.fst (enum l) = range l.length := by
   simp only [enum, enumFrom_map_fst, range_eq_range']
 
-@[simp]
+@[deprecated zipIdx_map_fst (since := "2025-01-21"), simp]
 theorem enum_map_snd (l : List α) : map Prod.snd (enum l) = l :=
   enumFrom_map_snd _ _
 
+@[deprecated zipIdx_map (since := "2025-01-21")]
 theorem enum_map (l : List α) (f : α → β) : (l.map f).enum = l.enum.map (Prod.map id f) :=
   enumFrom_map _ _ _
 
+@[deprecated zipIdx_append (since := "2025-01-21")]
 theorem enum_append (xs ys : List α) : enum (xs ++ ys) = enum xs ++ enumFrom xs.length ys := by
   simp [enum, enumFrom_append]
 
+@[deprecated zipIdx_eq_zip_range' (since := "2025-01-21")]
 theorem enum_eq_zip_range (l : List α) : l.enum = (range l.length).zip l :=
   zip_of_prod (enum_map_fst _) (enum_map_snd _)
 
-@[simp]
+@[deprecated unzip_zipIdx_eq_prod (since := "2025-01-21"), simp]
 theorem unzip_enum_eq_prod (l : List α) : l.enum.unzip = (range l.length, l) := by
   simp only [enum_eq_zip_range, unzip_zip, length_range]
 
+@[deprecated zipIdx_eq_cons_iff (since := "2025-01-21")]
 theorem enum_eq_cons_iff {l : List α} :
     l.enum = x :: l' ↔ ∃ a as, l = a :: as ∧ x = (0, a) ∧ l' = enumFrom 1 as := by
   rw [enum, enumFrom_eq_cons_iff]
 
+@[deprecated zipIdx_eq_append_iff (since := "2025-01-21")]
 theorem enum_eq_append_iff {l : List α} :
     l.enum = l₁ ++ l₂ ↔
       ∃ l₁' l₂', l = l₁' ++ l₂' ∧ l₁ = l₁'.enum ∧ l₂ = l₂'.enumFrom l₁'.length := by
   simp [enum, enumFrom_eq_append_iff]
+
+end
 
 end List
